src3.0/Transforms/vmem2reg_opt_compose_props.v
@@ -1,6 +1,32 @@
 Require Import vellvm.
 Require Import ListSet.
+Require Import primitives.
+Require Import palloca_props.
+Require Import vmem2reg.
 Require Import vmem2reg_opt.
+
+(***************************************************************)
+
+Lemma lookupAL_map_iff: forall A f m id0 ac0,
+  lookupAL A (ListMap.map f m) id0 = Some ac0 <->
+    exists ac1, ac0 = f ac1 /\ lookupAL A m id0 = Some ac1.
+Proof.
+  induction m as [|[id1 v1] m]; simpl; intros.
+    split; intro J; try congruence.
+      destruct J as [ac1 [? J]]; congruence.
+
+    destruct_if.
+    split; intro J.
+      uniq_result. eauto.
+
+      destruct J as [ac1 [? ?]]; uniq_result; auto.
+Qed.
+
+Lemma action_dec: forall (ac1 ac2: action), {ac1 = ac2} + {ac1 <> ac2}.
+Proof. decide equality; auto using value_dec, typ_dec. Qed.
+
+Lemma id_action_dec: forall (ia1 ia2: id*action), {ia1 = ia2} + {ia1 <> ia2}.
+Proof. decide equality; auto using id_dec, action_dec. Qed.
 
 (***************************************************************)
 
@@ -61,71 +87,11 @@ end.
 
 (***************************************************************)
 
-Lemma in_dom__iff__in_rev_dom: forall i0 X (A:list (id*X)),
-  i0 `in` dom A <-> i0 `in` dom (rev A).
-Proof.
-  induction A as [|[] A]; simpl.
-    split; auto.
-
-    rewrite dom_app. simpl.
-    fsetdec.
-Qed.
-
-Lemma uniq__iff__uniq_rev: forall X (A:list (id*X)),
-  uniq A <-> uniq (rev A).
-Proof.
-  induction A as [|[] A]; simpl.
-    split; auto.
-
-    split; intro J.
-      inv J. 
-      apply uniq_app_iff.
-      split. apply IHA; auto.
-      split. apply uniq_cons; auto.
-        apply disjoint_one_r. 
-        intro J. apply H3.
-        eapply in_dom__iff__in_rev_dom; eauto.
-
-      apply uniq_app_iff in J.
-      destruct J as [J1 [J2 J3]].
-      apply uniq_cons; auto.
-        apply IHA; auto.
-
-        apply disjoint_one_r in J3. 
-        intro J. apply J3.
-        apply in_dom__iff__in_rev_dom in J; auto.
-Qed.
-
 Definition ids_in_stld_state (st:stld_state) : list id :=
 match st with
 | STLD_store i1 _ => [i1]
 | _ => nil
 end.
-
-Lemma In_fst__in_dom: forall X (A:list (id*X)) i0,
-  In i0 (List.map fst A) <-> i0 `in` dom A.
-Proof.
-  induction A as [|[] A]; simpl; intros; auto.
-    split; intro J.
-      inv J. fsetdec.
-
-    split; intro J.
-      destruct J as [J | J]; subst; auto.
-        apply IHA in J; auto.
-
-      apply AtomSetFacts.add_iff in J.
-      destruct J as [J | J]; subst; auto.
-        apply IHA in J; auto.
-Qed.
-
-Lemma NoDup_fst__uniq: forall X (A:list (id*X)) (Huniq: NoDup (List.map fst A)), 
-  uniq A.
-Proof.
-  induction A as [|[] A]; simpl; intros; auto.
-    inv Huniq.
-    apply uniq_cons; auto.
-      intro J. apply H1. apply In_fst__in_dom; auto.
-Qed.
 
 Lemma find_stld_pairs_cmds_aux__uniq: forall pid cs s acs
   (Huniq : NoDup (getCmdsLocs cs ++ ids_in_stld_state s ++ List.map fst acs)),
@@ -281,12 +247,1393 @@ Qed.
 
 (***************************************************************)
 
+Lemma find_init_stld_inl_remove_neq_spec: forall dones id' pid cs1 v2 id2 cs2
+  (Hneq: id2 <> id')
+  (Hst : Some (inl (id2, v2, cs2)) = find_init_stld cs1 pid dones),
+  Some (inl (id2, v2, remove_cmds id' cs2)) =
+             find_init_stld (remove_cmds id' cs1) pid dones.
+Proof.
+  induction cs1 as [|c cs1]; simpl; intros.
+    congruence.
+
+    destruct (id_dec (getCmdLoc c) id'); subst; simpl.
+    Case "1".
+      destruct c; auto.
+      SCase "1.1".
+        destruct_if; auto.
+        destruct_if; auto.
+      SCase "1.2".
+        destruct value2; auto.
+        destruct_if; auto.
+        destruct_if; auto.
+          simpl in Hneq. congruence.
+    Case "2".
+      destruct c; auto.
+      SCase "1.1".
+        destruct_if; auto.
+        destruct_if; auto.
+      SCase "1.2".
+        destruct value2; auto.
+        destruct_if; auto.
+        destruct_if; auto.
+Qed.
+
+Lemma find_next_stld_inr_remove_neq_spec: forall id' pid cs1 v3 id3
+  (Hneq: id3 <> id')
+  (Hst : Some (inr (id3, v3)) = find_next_stld cs1 pid),
+  Some (inr (id3, v3)) = find_next_stld (remove_cmds id' cs1) pid.
+Proof.
+  induction cs1 as [|c cs1]; simpl; intros; auto.
+    destruct (id_dec (getCmdLoc c) id'); subst; simpl.
+    Case "1".
+      destruct c; auto.
+      SCase "1.1".
+        destruct value1; auto.
+        destruct_if; auto.
+      SCase "1.2".
+        destruct value2; auto.
+        destruct_if; auto.
+          simpl in Hneq. congruence.
+    Case "2".
+      destruct c; auto.
+      SCase "2.1".
+        destruct value1; auto.
+        destruct_if; auto.
+      SCase "2.2".
+        destruct value2; auto.
+        destruct_if; auto.
+Qed.
+
+Lemma find_init_stld_inl_in: forall (cs5 : cmds) (id' : atom) (v0 : value)
+  (cs0 : cmds) (dones : list id) pinfo
+  (Hfind : ret inl (id', v0, cs0) = find_init_stld cs5 (PI_id pinfo) dones),
+  In id' (getCmdsLocs cs5).
+Proof.
+  intros.
+  apply find_init_stld_inl_spec in Hfind.
+  destruct Hfind as [cs1 [ty1 [al1 Hst]]]; subst.
+  rewrite getCmdsLocs_app. simpl. xsolve_in_list.
+Qed.
+
+Lemma find_next_stld_inr_in: forall (cs5 : cmds) (id' : atom) (v0 : value)
+  pinfo
+  (Hfind : ret inr (id', v0) = find_next_stld cs5 (PI_id pinfo)),
+  In id' (getCmdsLocs cs5).
+Proof.
+  intros.
+  apply find_next_stld_inr_spec in Hfind.
+  destruct Hfind as [cs1 [cs2 [ty1 [al1 [J1 J2]]]]]; subst.
+  rewrite getCmdsLocs_app. simpl. xsolve_in_list.
+Qed.
+
+Lemma find_st_ld__sas_in: forall cs0 i0 v cs dones pinfo
+  (Hst : ret inl (i0, v, cs) = find_init_stld cs0 (PI_id pinfo) dones) v0
+  (i1 : id) (Hld : ret inr (i1, v0) = find_next_stld cs (PI_id pinfo)),
+  In i1 (getCmdsLocs cs0).
+Proof.
+  intros.
+  apply find_init_stld_inl_spec in Hst.
+  destruct Hst as [cs1 [ty1 [al1 Hst]]]; subst.
+  apply find_next_stld_inr_in in Hld.
+  rewrite getCmdsLocs_app. simpl. xsolve_in_list.
+Qed.
+
+Lemma find_next_stld_inr_spec': forall pinfo i1 v0 cs
+ (H: ret inr (i1, v0) = find_next_stld cs (PI_id pinfo)),
+ exists cs1, exists cs2, exists ty, exists al,
+   cs = cs1 ++
+          insn_store i1 ty v0 (value_id (PI_id pinfo)) al :: cs2 /\
+   load_in_cmds (PI_id pinfo) cs1 = false /\
+   store_in_cmds (PI_id pinfo) cs1 = false.
+Proof.
+  induction cs; simpl; intros.
+    congruence.
+
+    destruct a; try find_next_stld_spec_tac.
+      destruct value1; try solve [find_next_stld_spec_tac].
+      destruct_if.
+        find_next_stld_spec_tac.
+        destruct H2.
+        split; auto. 
+        split.
+          simpl_env.
+          apply load_in_cmds_merge.
+          split; auto. 
+            unfold load_in_cmds. simpl.
+            destruct (id_dec id0 (PI_id pinfo)); try solve [auto | congruence].
+
+          simpl_env.
+          apply store_in_cmds_merge.
+          split; auto. 
+
+      destruct value2; try solve [find_next_stld_spec_tac].
+      repeat (destruct_if; try solve [find_next_stld_spec_tac]).
+      exists nil. exists cs. exists typ5. exists align5.
+      split; auto.
+
+      find_next_stld_spec_tac.
+      destruct H2.      
+      repeat split; auto.
+        unfold store_in_cmds. simpl.
+        destruct (id_dec id0 (PI_id pinfo)); try solve [auto | congruence].
+Qed.
+
+Lemma find_st_ld__sas_spec: forall cs0 i0 v cs dones pinfo
+  (Hst : ret inl (i0, v, cs) = find_init_stld cs0 (PI_id pinfo) dones) v0
+  (i1 : id) (Hld : ret inr (i1, v0) = find_next_stld cs (PI_id pinfo)),
+  exists cs1 : list cmd, exists ty0 : typ, exists al0 : align,
+    cs0 = cs1 ++ insn_store i0 ty0 v (value_id (PI_id pinfo)) al0 :: cs /\
+  exists cs2 : list cmd, exists cs3 : list cmd,
+    exists ty1 : typ, exists al1 : align,
+    cs = cs2 ++ insn_store i1 ty1 v0 (value_id (PI_id pinfo)) al1 :: cs3 /\
+    load_in_cmds (PI_id pinfo) cs2 = false /\
+    store_in_cmds (PI_id pinfo) cs2 = false.
+Proof.
+  intros.
+  apply find_init_stld_inl_spec in Hst.
+  destruct Hst as [cs1 [ty1 [al1 Hst]]]; subst.
+  apply find_next_stld_inr_spec' in Hld.
+  destruct Hld as [cs2 [cs3 [ty2 [al2 [Hld [J1 J2]]]]]]; subst.
+  eauto 11.
+Qed.
+
+Require Import trans_tactic.
+
+Lemma find_next_stld_inl_spec': forall pid i1 cs
+ (H: ret inl i1 = find_next_stld cs pid),
+ exists cs1, exists cs2, exists ty, exists al,
+   cs = cs1 ++
+          insn_load i1 ty (value_id pid) al :: cs2 /\
+   store_in_cmds pid cs1 = false /\
+   load_in_cmds pid cs1 = false.
+Proof.
+  induction cs; simpl; intros.
+    congruence.
+
+    destruct a; try find_next_stld_spec_tac.
+      destruct value1; try solve [find_next_stld_spec_tac].
+      destruct_if.
+        exists nil. exists cs. exists typ5. exists align5.
+        split; auto.
+
+        find_next_stld_spec_tac.
+        destruct H2. split; auto.
+        split.
+          apply store_in_cmds_false_cons_intro; auto.
+          apply load_in_cmds_false_cons_intro; auto.
+            simpl. destruct_dec.
+ 
+      destruct value2; try solve [find_next_stld_spec_tac].
+      destruct_if; try find_next_stld_spec_tac.
+        destruct H2.
+        split; auto. 
+        split.
+          simpl_env.
+          apply store_in_cmds_merge.
+          split; auto. 
+            unfold store_in_cmds. simpl.
+            destruct_dec. 
+          apply load_in_cmds_false_cons_intro; auto.
+Qed.
+
+Lemma find_st_ld__las_spec: forall cs0 i0 v cs dones pinfo
+  (Hst : ret inl (i0, v, cs) = find_init_stld cs0 (PI_id pinfo) dones) 
+  (i1 : id) (Hld : ret (inl i1) = find_next_stld cs (PI_id pinfo)),
+  exists cs1 : list cmd, exists ty0 : typ, exists al0 : align,
+    cs0 = cs1 ++ insn_store i0 ty0 v (value_id (PI_id pinfo)) al0 :: cs /\
+  exists cs2, exists cs3, exists ty1, exists al1,
+    cs = cs2 ++ insn_load i1 ty1 (value_id (PI_id pinfo)) al1 :: cs3 /\
+    store_in_cmds (PI_id pinfo) cs2 = false /\
+    load_in_cmds (PI_id pinfo) cs2 = false.
+Proof.
+  intros.
+  apply find_init_stld_inl_spec in Hst.
+  destruct Hst as [cs1 [ty1 [al1 Hst]]]; subst.
+  apply find_next_stld_inl_spec' in Hld.
+  destruct Hld as [cs2 [cs3 [ty2 [al2 [Hld [J1 J2]]]]]]; subst.
+  eauto 11.
+Qed.
+
+Lemma find_next_stld_inl_remove_neq_spec: forall id' pid cs1 id3
+  (Hneq: id3 <> id')
+  (Hst : Some (inl id3) = find_next_stld cs1 pid),
+  Some (inl id3) = find_next_stld (remove_cmds id' cs1) pid.
+Proof.
+  induction cs1 as [|c cs1]; simpl; intros; auto.
+    destruct (id_dec (getCmdLoc c) id'); subst; simpl.
+    Case "1".
+      destruct c; auto.
+      SCase "1.1".
+        destruct value1; auto.
+        destruct_if; auto.
+          simpl in Hneq. congruence.
+      SCase "1.2".
+        destruct value2; auto.
+        destruct_if; auto.
+    Case "2".
+      destruct c; auto.
+      SCase "2.1".
+        destruct value1; auto.
+        destruct_if; auto.
+      SCase "2.2".
+        destruct value2; auto.
+        destruct_if; auto.
+Qed.
+
+Lemma find_init_stld_inr_remove_neq_spec: forall dones id' pid cs1 v2 cs2
+  (Hneq: pid <> id')
+  (Hst : Some (inr (v2, cs2)) = find_init_stld cs1 pid dones),
+  Some (inr (v2, remove_cmds id' cs2)) =
+             find_init_stld (remove_cmds id' cs1) pid dones.
+Proof.
+  induction cs1 as [|c cs1]; simpl; intros.
+    congruence.
+
+    destruct (id_dec (getCmdLoc c) id'); subst; simpl.
+    Case "1".
+      destruct c; auto.
+      SCase "1.1".
+        destruct_if; auto.
+        destruct_if; auto.
+          simpl in Hneq. congruence.
+      SCase "1.2".
+        destruct value2; auto.
+        destruct_if; auto.
+        destruct_if; auto.
+    Case "2".
+      destruct c; auto.
+      SCase "1.1".
+        destruct_if; auto.
+        destruct_if; auto.
+      SCase "1.2".
+        destruct value2; auto.
+        destruct_if; auto.
+        destruct_if; auto.
+Qed.
+        
+Lemma find_init_stld_inl_subst_spec: forall dones id' v' pid cs1 v2 id2 cs2
+  (Hnused: used_in_value pid v' = false) (Hneq: id' <> pid) 
+  (Hst : Some (inl (id2, v2, cs2)) = find_init_stld cs1 pid dones),
+  Some (inl (id2, subst_value id' v' v2, List.map (subst_cmd id' v') cs2)) =
+             find_init_stld (List.map (subst_cmd id' v') cs1) pid dones.
+Proof.
+  induction cs1 as [|c cs1]; simpl; intros.
+    congruence.
+
+    destruct c; simpl; auto.
+    Case "1.1".
+      destruct_if; auto.
+      destruct_if; auto.
+    Case "1.2".
+      destruct value2; simpl; auto.
+      destruct_if; auto.
+      destruct_if; auto.
+      destruct (id_dec id0 id'); subst.
+        destruct v'.
+          simpl in Hnused.
+          destruct_if. 
+            destruct_if; auto. congruence.
+            destruct_if; auto. 
+              destruct (id_dec id0 id0); simpl in Hnused; try congruence.
+
+          destruct_if; auto. 
+            congruence.
+           
+        destruct_if; auto.
+Qed.
+
+Lemma find_next_stld_inr_subst_spec: forall id' v' pid cs1 v3 id3
+  (Hnused: used_in_value pid v' = false) (Hneq: id' <> pid) 
+  (Hst : Some (inr (id3, v3)) = find_next_stld cs1 pid),
+  Some (inr (id3, v3 {[v' // id']})) = 
+    find_next_stld (List.map (subst_cmd id' v') cs1) pid.
+Proof.
+  induction cs1 as [|c cs1]; simpl; intros.
+    congruence.
+
+    destruct c; simpl; auto.
+    Case "1.1".
+      destruct value1; simpl; auto.
+      destruct_if; auto.
+      destruct (id_dec id0 id'); subst.
+        destruct v'; auto.
+          simpl in Hnused.
+          destruct_if; auto. 
+            destruct (id_dec id0 id0); simpl in Hnused; try congruence.
+
+        destruct_if; auto. congruence.
+    Case "1.2".
+      destruct value2; simpl; auto.
+      destruct (id_dec id0 id'); subst.
+        destruct v'.
+          simpl in Hnused.
+          destruct_if. 
+            destruct_if; auto. congruence.
+            destruct_if; auto. 
+              destruct (id_dec id0 id0); simpl in Hnused; try congruence.
+
+          destruct_if; auto. 
+            congruence.
+           
+        destruct_if; auto.
+Qed.
+
+Lemma find_next_stld_inl_subst_spec: forall id' v' pid cs1 id3
+  (Hnused: used_in_value pid v' = false) (Hneq: id' <> pid) 
+  (Hst : Some (inl id3) = find_next_stld cs1 pid),
+  Some (inl id3) = find_next_stld (List.map (subst_cmd id' v') cs1) pid.
+Proof.
+  induction cs1 as [|c cs1]; simpl; intros.
+    congruence.
+
+    destruct c; simpl; auto.
+    Case "1.1".
+      destruct value1; simpl; auto.
+      destruct (id_dec id0 id'); subst.
+        destruct v'.
+          simpl in Hnused.
+          destruct (id_dec pid id0); subst.
+            destruct (id_dec id0 id0); simpl in Hnused; try congruence.
+            destruct_if; auto. congruence.
+          destruct_if; auto. congruence.
+        destruct_if; auto. 
+    Case "1.2".
+      destruct value2; simpl; auto.
+      destruct (id_dec id0 id'); subst.
+        destruct v'.
+          simpl in Hnused.
+          destruct_if. 
+          destruct_if; auto. 
+            destruct (id_dec id0 id0); simpl in Hnused; try congruence.
+
+          destruct_if; auto. 
+        destruct_if; auto.
+Qed.
+
+Lemma find_init_stld_inr_subst_spec: forall dones id' v' pid cs1 v2 cs2
+  (Hnused: used_in_value pid v' = false)
+  (Hst : Some (inr (v2, cs2)) = find_init_stld cs1 pid dones),
+  Some (inr (subst_value id' v' v2, List.map (subst_cmd id' v') cs2)) =
+             find_init_stld (List.map (subst_cmd id' v') cs1) pid dones.
+Proof.
+  induction cs1 as [|c cs1]; simpl; intros.
+    congruence.
+
+    destruct c; simpl; auto.
+    Case "1.1".
+      destruct_if; auto.
+      destruct_if; auto.
+    Case "1.2".
+      destruct value2; simpl; auto.
+      destruct (id_dec id0 id'); subst.
+        destruct v'.
+          simpl in Hnused.
+          destruct_if; auto.
+          destruct_if; auto. 
+          destruct_if; auto. 
+            destruct (id_dec id0 id0); simpl in Hnused; try congruence.
+
+          destruct_if; auto. 
+          destruct_if; auto. 
+           
+        destruct_if; auto.
+        destruct_if; auto.
+Qed.
+
+Lemma find_init_stld_inl_doesnt_use_pid: forall pinfo l5 ps5 cs5 tmn5 dones
+  (Hwfpi: WF_PhiInfo pinfo)
+  (Huniq : uniqFdef (PI_f pinfo)) s m (HwfF: wf_fdef s m (PI_f pinfo))
+  (HBinF : blockInFdefB (l5, stmts_intro ps5 cs5 tmn5) (PI_f pinfo) = true)
+  id' v' cs0
+  (Hst: Some (inl (id', v', cs0)) = find_init_stld cs5 (PI_id pinfo) dones),
+  used_in_value (PI_id pinfo) v' = false /\ id' <> (PI_id pinfo).
+Proof.
+  intros.
+  apply find_init_stld_inl_spec in Hst.
+  destruct Hst as [cs1 [ty [al EQ]]]; subst.
+  split.
+    eapply IngetCmdsIDs__lookupCmdViaIDFromFdef in HBinF; eauto 1 using in_middle.
+    apply WF_PhiInfo_spec4 with (v0:=v') in HBinF; auto.
+
+    apply WF_PhiInfo_spec10 in HBinF; auto.
+Qed.
+
+Lemma find_st_ld_las_doesnt_use_pid: forall pinfo l5 ps5 cs5 tmn5 dones
+  (Hwfpi: WF_PhiInfo pinfo)
+  (Huniq : uniqFdef (PI_f pinfo)) s m (HwfF: wf_fdef s m (PI_f pinfo))
+  (HBinF : blockInFdefB (l5, stmts_intro ps5 cs5 tmn5) (PI_f pinfo) = true)
+  id' v' cs0 id0
+  (Hst: Some (inl (id0, v', cs0)) = find_init_stld cs5 (PI_id pinfo) dones)
+  (Hld: ret inl id' = find_next_stld cs0 (PI_id pinfo)),
+  used_in_value (PI_id pinfo) v' = false /\ id' <> (PI_id pinfo).
+Proof.
+  intros.
+  eapply find_st_ld__las_spec in Hst; eauto.
+  destruct Hst as [cs1 [ty [al [EQ [cs2 [cs3 [ty1 [al1 [EQ1 [J1 J2]]]]]]]]]]; 
+    subst.
+  split.
+    eapply IngetCmdsIDs__lookupCmdViaIDFromFdef in HBinF; eauto 1 using in_middle.
+    apply WF_PhiInfo_spec4 with (v0:=v') in HBinF; auto.
+
+    match goal with
+    | H: context [?A ++ ?b :: ?C ++ ?d :: ?E] |- _ =>
+      rewrite_env ((A++b::C)++d::E) in H;
+      apply WF_PhiInfo_spec10 in H; auto
+    end.
+Qed.
+
+Lemma find_st_ld_laa_doesnt_use_pid: forall pinfo l5 ps5 cs5 tmn5 dones
+  (Hwfpi: WF_PhiInfo pinfo)
+  (Huniq : uniqFdef (PI_f pinfo)) s m (HwfF: wf_fdef s m (PI_f pinfo))
+  (HBinF : blockInFdefB (l5, stmts_intro ps5 cs5 tmn5) (PI_f pinfo) = true)
+  id' v' cs0
+  (Hst: Some (inr (v', cs0)) = find_init_stld cs5 (PI_id pinfo) dones)
+  (Hld: ret inl id' = find_next_stld cs0 (PI_id pinfo)),
+  used_in_value (PI_id pinfo) v' = false /\ id' <> (PI_id pinfo).
+Proof.
+  intros.
+  apply find_init_stld_inr_spec in Hst.
+  destruct Hst as [cs1 [ty1 [num1 [al1 [EQ Hst]]]]]; subst.
+  apply find_next_stld_inl_spec' in Hld.
+  destruct Hld as [cs2 [cs3 [ty2 [al2 [Hld [J1 J2]]]]]]; subst.
+  split.
+    simpl. auto.
+
+    match goal with
+    | H: context [?A ++ ?b :: ?C ++ ?d :: ?E] |- _ =>
+      rewrite_env ((A++b::C)++d::E) in H;
+      apply WF_PhiInfo_spec10 in H; auto
+    end.
+Qed.
+
+Lemma find_init_stld_inl_intro_aux: forall id0 v cs4 ty0 al0 pid dones cs3
+  (Hinc: incl (getCmdsLocs cs3) dones) 
+  (Huniq: NoDup (dones ++ id0 :: getCmdsLocs cs4)),
+  Some (inl (id0, v, cs4)) =
+     find_init_stld
+       (cs3 ++ insn_store id0 ty0 v (value_id pid) al0 :: cs4) pid
+       dones.
+Proof.
+  induction cs3 as [|c3 cs3]; simpl; intros.
+    destruct_if.
+      eapply NoDup_disjoint' in Huniq; eauto.
+      contradict Huniq; simpl; auto.
+
+      destruct_if. congruence.
+
+    destruct c3; try (apply IHcs3; eauto with datatypes v62).
+      destruct_if; try (apply IHcs3; eauto with datatypes v62).
+      destruct_if; try (apply IHcs3; eauto with datatypes v62).
+        clear HeqR.
+        contradict n. apply Hinc. simpl; auto.
+
+      destruct value2 as [qid|]; try (apply IHcs3; eauto with datatypes v62).
+      destruct_if; try (apply IHcs3; eauto with datatypes v62).
+      destruct_if; try (apply IHcs3; eauto with datatypes v62).
+        clear HeqR.
+        contradict n. apply Hinc. simpl; auto.
+Qed.
+
+Lemma find_init_stld_inl_intro: forall id0 v cs4 ty0 al0 pid cs3
+  (Huniq: NoDup (getCmdsLocs cs3 ++ id0 :: getCmdsLocs cs4)),
+  Some (inl (id0, v, cs4)) =
+     find_init_stld
+       (cs3 ++ insn_store id0 ty0 v (value_id pid) al0 :: cs4) pid
+       (getCmdsLocs cs3).
+Proof.
+  intros.
+  apply find_init_stld_inl_intro_aux; auto with datatypes v62.
+Qed.
+
+Lemma find_init_stld_inr_intro_aux: forall cs4 t num0 al0 pid dones cs3
+  (Hinc: incl (getCmdsLocs cs3) dones) 
+  (Huniq: NoDup (dones ++ pid :: getCmdsLocs cs4)),
+  Some (inr (value_const (const_undef t), cs4)) =
+     find_init_stld
+       (cs3 ++ insn_alloca pid t num0 al0 :: cs4) pid
+       dones.
+Proof.
+  induction cs3 as [|c3 cs3]; simpl; intros.
+    destruct_if.
+      eapply NoDup_disjoint' in Huniq; eauto.
+      contradict Huniq; simpl; auto.
+
+      destruct_if. congruence.
+
+    destruct c3; try (apply IHcs3; eauto with datatypes v62).
+      destruct_if; try (apply IHcs3; eauto with datatypes v62).
+      destruct_if; try (apply IHcs3; eauto with datatypes v62).
+        clear HeqR.
+        contradict n. apply Hinc. simpl; auto.
+
+      destruct value2 as [qid|]; try (apply IHcs3; eauto with datatypes v62).
+      destruct_if; try (apply IHcs3; eauto with datatypes v62).
+      destruct_if; try (apply IHcs3; eauto with datatypes v62).
+        clear HeqR.
+        contradict n. apply Hinc. simpl; auto.
+Qed.
+
+Lemma find_init_stld_inr_intro: forall cs4 t num0 al0 pid cs3
+  (Huniq: NoDup (getCmdsLocs cs3 ++ pid :: getCmdsLocs cs4)),
+  Some (inr (value_const (const_undef t), cs4)) =
+     find_init_stld
+       (cs3 ++ insn_alloca pid t num0 al0 :: cs4) pid
+       (getCmdsLocs cs3).
+Proof.
+  intros.
+  apply find_init_stld_inr_intro_aux; auto with datatypes v62.
+Qed.
+
+Lemma find_next_stld_strengthen: forall cs2 pid cs1 
+  (Hnst: store_in_cmds pid cs1 = false)
+  (Hnld: load_in_cmds pid cs1 = false),
+  find_next_stld cs2 pid = find_next_stld (cs1++cs2) pid.
+Proof.
+  induction cs1 as [|c cs1]; simpl; intros; auto.
+    apply store_in_cmds_false_cons_inv in Hnst.
+    destruct Hnst as [Hnst1 Hnst2].
+    apply load_in_cmds_false_cons_inv in Hnld.
+    destruct Hnld as [Hnld1 Hnld2].
+    destruct c; auto.
+      destruct value1; auto.
+      destruct_if.
+      simpl in Hnld1.
+      destruct (id_dec id0 id0); simpl in Hnld1; try congruence.
+
+      destruct value2; auto.
+      destruct_if.
+      simpl in Hnst1.
+      destruct (id_dec id0 id0); simpl in Hnst1; try congruence.   
+Qed.
+
+Lemma find_init_stld_inl_in': forall (cs5 : cmds) (id' : atom) (v0 : value)
+  (dones : list id) pinfo cs01 c0 cs02
+  (Hfind : ret inl (id', v0, cs01 ++ c0 :: cs02) = 
+             find_init_stld cs5 (PI_id pinfo) dones),
+  In c0 cs5.
+Proof.
+  intros.
+  apply find_init_stld_inl_spec in Hfind.
+  destruct Hfind as [cs1 [ty1 [al1 Hst]]]; subst.
+  xsolve_in_list.
+Qed.
+
+Lemma find_next_stld_inr_intro: forall c0 cs01 pid cs02
+  (Hnst : store_in_cmds pid cs01 = false)
+  (Hst : store_in_cmd pid c0 = true) (Hnld : load_in_cmds pid cs01 = false),
+  exists v1 : value,
+    ret inr (getCmdLoc c0, v1) = find_next_stld (cs01 ++ c0 :: cs02) pid.
+Proof.
+  intros.
+  rewrite <- find_next_stld_strengthen; auto.
+  destruct c0; tinv Hst.
+  destruct value2; tinv Hst.
+  simpl in Hst. simpl.
+  destruct (id_dec id0 pid); subst; tinv Hst.
+  destruct_if; eauto.
+    congruence.
+Qed.
+
+Lemma find_next_stld_inl_intro: forall c0 cs01 pid cs02
+  (Hnst : store_in_cmds pid cs01 = false)
+  (Hld : load_in_cmd pid c0 = true) (Hnld : load_in_cmds pid cs01 = false),
+  ret inl (getCmdLoc c0) = find_next_stld (cs01 ++ c0 :: cs02) pid.
+Proof.
+  intros.
+  rewrite <- find_next_stld_strengthen; auto.
+  destruct c0; tinv Hld.
+  destruct value1; tinv Hld.
+  simpl in Hld. simpl.
+  destruct (id_dec id0 pid); subst; tinv Hld.
+  destruct_if; eauto.
+    congruence.
+Qed.
+
+Lemma list_subst_actions_app_inv: forall id0 ac0 acs acs1' acs2'
+  (Heq: ListComposedPass.subst_actions id0 ac0 acs = acs1' ++ acs2'),
+  exists acs1, exists acs2,
+    acs = acs1 ++ acs2 /\ 
+    ListComposedPass.subst_actions id0 ac0 acs1 = acs1' /\
+    ListComposedPass.subst_actions id0 ac0 acs2 = acs2'.
+Proof.
+  unfold ListComposedPass.subst_actions.
+  intros.
+  destruct (action2value ac0).
+    apply map_app_inv; auto.
+    subst. eauto.
+Qed.
+
+(***************************************************************)
+
+Definition loads_must_be_in_pre (acs: AssocList action) (pid:id) (cs:cmds)
+  : Prop :=
+Forall (fun c => load_in_cmd pid c = true -> getCmdLoc c `in` dom acs) cs.
+
+Lemma filter_pres_loads_must_be_in_pre: forall acs check pid cs
+  (Hnld: loads_must_be_in_pre acs pid cs),
+  loads_must_be_in_pre acs pid (filter check cs).
+Proof.
+  induction 1; simpl; intros.
+    constructor.
+
+    destruct_if.
+    constructor; auto.
+Qed.
+
+Lemma no_loads__loads_must_be_in_pre: forall pid acs cs
+  (H: load_in_cmds pid cs = false),
+  loads_must_be_in_pre acs pid cs.
+Proof.
+  induction cs as [|c cs]; intros.
+    constructor.
+
+    apply load_in_cmds_false_cons_inv in H.
+    destruct H as [H1 H2].
+    constructor.
+      intros. congruence.
+      apply IHcs; auto.
+Qed.
+
+Lemma loads_must_be_in_pre_merge: forall acs pid cs1 cs2
+  (Hlds1: loads_must_be_in_pre acs pid cs1) 
+  (Hlds2: loads_must_be_in_pre acs pid cs2),
+  loads_must_be_in_pre acs pid (cs1 ++ cs2).
+Proof.
+  unfold loads_must_be_in_pre.
+  intros.
+  apply Forall_app; auto.
+Qed.
+
+Lemma loads_must_be_in_pre_load_in_cmds_false__loads_must_be_in_pre: 
+  forall acs pid cs1 cs2
+  (Hlds1: loads_must_be_in_pre acs pid cs1) 
+  (Hlds2: load_in_cmds pid cs2 = false),
+  loads_must_be_in_pre acs pid (cs1 ++ cs2).
+Proof.
+  intros.
+  apply loads_must_be_in_pre_merge; auto.
+  apply no_loads__loads_must_be_in_pre; auto.
+Qed.
+
+Lemma remove_pres_loads_must_be_in_pre: forall id' ac' actions pid cs
+  (Hld: loads_must_be_in_pre ((id', ac') :: actions) pid cs),
+  loads_must_be_in_pre actions pid 
+    (filter (fun c : cmd => negb (id_dec (getCmdLoc c) id')) cs).
+Proof.
+  induction 1; simpl; intros.
+    constructor.
+
+    destruct_dec; simpl.
+      constructor; auto.
+        intros Heq. apply H in Heq.
+        simpl in Heq. fsetdec.
+Qed.
+
+Lemma loads_must_be_in_nil__no_loads: forall pid cs 
+  (H: loads_must_be_in_pre nil pid cs), load_in_cmds pid cs = false.
+Proof.
+  induction 1; simpl; auto.
+    apply load_in_cmds_false_cons_intro; auto.
+      case_eq (load_in_cmd pid x); auto.
+        intro Heq.
+        apply H in Heq. fsetdec.
+Qed.
+
+Lemma loads_must_be_in_pre_append: forall acs pid cs3 c
+  (Hlds: loads_must_be_in_pre acs pid cs3) (Hld: load_in_cmd pid c = false),
+  loads_must_be_in_pre acs pid (cs3 ++ [c]).
+Proof.
+  intros.
+  apply Forall_forall.
+  intros x Hinx H.
+  destruct_in Hinx.
+    eapply Forall_forall in Hlds; eauto.
+    destruct_in Hinx. congruence.
+Qed.
+
+Lemma loads_must_be_in_pre_weaken: forall acs1 acs2 pid cs 
+  (Hlds: loads_must_be_in_pre acs2 pid cs),
+  loads_must_be_in_pre (acs1++acs2) pid cs.
+Proof.
+  induction 1; constructor; auto.
+    intro Heq. apply H in Heq. rewrite dom_app. auto.
+Qed.
+
+Lemma loads_must_be_in_pre_append': forall ac acs pid cs3 c
+  (Hlds: loads_must_be_in_pre acs pid cs3) (Hld: load_in_cmd pid c = true)
+  (Heq: fst ac = getCmdLoc c),
+  loads_must_be_in_pre ([ac]++acs) pid (cs3 ++ [c]).
+Proof.
+  intros.
+  apply Forall_forall.
+  intros x Hinx H.
+  destruct_in Hinx.
+    eapply Forall_forall in Hlds; eauto.
+    apply Hlds in H. simpl_env. auto.
+
+    destruct_in Hinx. 
+      destruct ac. simpl in *. subst. auto.
+Qed.
+
+Lemma loads_must_be_in_pre_rev: forall acs pid cs
+  (Hwf: loads_must_be_in_pre (rev acs) pid cs),
+  loads_must_be_in_pre acs pid cs.
+Proof.
+  unfold loads_must_be_in_pre. intros.
+  apply Forall_forall. intros x Hinx Heq.
+  eapply Forall_forall in Hwf; eauto.
+  apply Hwf in Heq.
+  apply binds_In_inv in Heq.
+  destruct Heq as [ac Heq].
+  apply binds_In with (a:=ac); auto.
+  unfold binds in *.
+  apply in_rev; auto.
+Qed.
+
+(***************************************************************)
+
+Definition wf_cs_action (cs:cmds) (pid:id) (elt:id * action): Prop :=
+let '(id', ac') := elt in
+match ac' with
+| AC_remove =>  
+    exists v0, exists cs0, exists id1, exists v1, exists dones,
+      Some (inl (id', v0, cs0)) = find_init_stld cs pid dones /\
+      Some (inr (id1, v1)) = find_next_stld cs0 pid
+| AC_vsubst v' =>  
+    exists id0, exists cs0, exists dones,
+      Some (inl (id0, v', cs0)) = find_init_stld cs pid dones /\
+      Some (inl id') = find_next_stld cs0 pid
+| AC_tsubst t' =>
+    exists cs0, exists dones,
+      Some (inr (value_const (const_undef t'), cs0)) = 
+        find_init_stld cs pid dones /\
+      Some (inl id') = find_next_stld cs0 pid
+end.
+
+(***************************************************************)
+
+Definition wf_cs_action_pre (acs: AssocList action) (cs:cmds) (pid:id) 
+  (elt:id * action): Prop :=
+let '(id', ac') := elt in
+match ac' with
+| AC_remove =>  
+    exists v0, exists cs01, exists c0, exists cs02, exists dones,    
+      Some (inl (id', v0, cs01 ++ c0 :: cs02)) = find_init_stld cs pid dones /\
+      store_in_cmds pid cs01 = false /\
+      store_in_cmd pid c0 = true /\ loads_must_be_in_pre acs pid cs01
+| AC_vsubst v' =>  
+    exists id0, exists cs01, exists c0, exists cs02, exists dones,    
+      Some (inl (id0, v', cs01 ++ c0 :: cs02)) = find_init_stld cs pid dones /\
+      store_in_cmds pid cs01 = false /\ getCmdLoc c0 = id' /\
+      load_in_cmd pid c0 = true /\ loads_must_be_in_pre acs pid cs01
+| AC_tsubst t' =>
+    exists cs01, exists c0, exists cs02, exists dones,
+      Some (inr (value_const (const_undef t'), cs01 ++ c0 :: cs02)) = 
+        find_init_stld cs pid dones /\
+      store_in_cmds pid cs01 = false /\ getCmdLoc c0 = id' /\
+      load_in_cmd pid c0 = true /\ loads_must_be_in_pre acs pid cs01
+end.
+
+Lemma wf_cs_action_nil__wf_cs_action: forall cs pid elt
+  (Hwf: wf_cs_action_pre nil cs pid elt), wf_cs_action cs pid elt.
+Proof.
+  unfold wf_cs_action_pre, wf_cs_action.
+  destruct elt as [id' [|v'|t']]; simpl; intros.
+  Case "1".
+    destruct Hwf as [v0 [cs01 [c0 [cs02 [dones [Hfind1 [Hnst [Hst Hnld]]]]]]]].
+    exists v0. exists (cs01 ++ c0 :: cs02). exists (getCmdLoc c0).
+    apply loads_must_be_in_nil__no_loads in Hnld.    
+    eapply find_next_stld_inr_intro with (cs02:=cs02) in Hnld; eauto.
+    destruct Hnld as [v1 Hnld]. eauto.
+  Case "2".
+    destruct Hwf 
+      as [id0 [cs01 [c0 [cs02 [dones [Hfind1 [Hnst [Heq [Hld Hnld]]]]]]]]]; subst.
+    exists id0. exists (cs01 ++ c0 :: cs02). exists dones.
+    apply loads_must_be_in_nil__no_loads in Hnld.    
+    eapply find_next_stld_inl_intro with (cs02:=cs02) in Hnld; eauto.
+  Case "3".
+    destruct Hwf 
+      as [cs01 [c0 [cs02 [dones [Hfind1 [Hnst [Heq [Hld Hnld]]]]]]]]; subst.
+    exists (cs01 ++ c0 :: cs02). exists dones.
+    apply loads_must_be_in_nil__no_loads in Hnld.    
+    eapply find_next_stld_inl_intro with (cs02:=cs02) in Hnld; eauto.
+Qed.
+
+Lemma wf_cs_action_pre_rev: forall acs cs pid ac 
+  (Hwf: wf_cs_action_pre (rev acs) cs pid ac),
+  wf_cs_action_pre acs cs pid ac.
+Proof.
+  unfold wf_cs_action_pre. intros.
+  destruct ac as [? []].
+    destruct Hwf as [v0 [cs01 [c0 [cs02 [dones [J1 [J2 [J3 J4]]]]]]]].
+    apply loads_must_be_in_pre_rev in J4. eauto 9.
+
+    destruct Hwf as [id0 [cs01 [c0 [cs02 [dones [J1 [J2 [J3 [J4 J5]]]]]]]]].
+    apply loads_must_be_in_pre_rev in J5. eauto 10.
+
+    destruct Hwf as [cs01 [c0 [cs02 [dones [J1 [J2 [J3 [J4 J5]]]]]]]].
+    apply loads_must_be_in_pre_rev in J5. eauto 9.
+Qed.
+
+Lemma wf_cs_action_pre_weaken: forall acs1 acs2 cs pid ac 
+  (Hwf: wf_cs_action_pre acs2 cs pid ac),
+  wf_cs_action_pre (acs1++acs2) cs pid ac.
+Proof.
+  unfold wf_cs_action_pre. intros.
+  destruct ac as [? []].
+    destruct Hwf as [v0 [cs01 [c0 [cs02 [dones [J1 [J2 [J3 J4]]]]]]]].
+    apply loads_must_be_in_pre_weaken with (acs1:=acs1) in J4. eauto 9.
+
+    destruct Hwf as [id0 [cs01 [c0 [cs02 [dones [J1 [J2 [J3 [J4 J5]]]]]]]]].
+    apply loads_must_be_in_pre_weaken with (acs1:=acs1) in J5. eauto 10.
+
+    destruct Hwf as [cs01 [c0 [cs02 [dones [J1 [J2 [J3 [J4 J5]]]]]]]].
+    apply loads_must_be_in_pre_weaken with (acs1:=acs1) in J5. eauto 9.
+Qed.
+
+(***************************************************************)
+Definition find_stld_pair_cmd' (pid:id) (acc:stld_state * AssocList action) 
+  (c:cmd) : stld_state * option (id * action) :=
+let '(st, actions) := acc in
+match c with
+| insn_alloca qid ty value5 align5 =>
+    if id_dec pid qid
+    then (STLD_alloca ty, None)
+    else (st, None)
+| insn_store sid typ5 v0 value2 align5 =>
+    match value2 with
+    | value_id qid =>
+       if id_dec pid qid
+       then 
+         match st with
+         | STLD_store sid' _ => (STLD_store sid v0, Some (sid', AC_remove))
+         | _ => (STLD_store sid v0, None)
+         end
+      else (st, None)
+    | value_const const5 => (st, None)
+    end
+| insn_load lid typ5 value1 align5 =>
+    match value1 with
+    | value_id qid =>
+       if id_dec pid qid
+       then 
+         match st with
+         | STLD_store _ v' => (st, Some (lid, AC_vsubst v'))
+         | STLD_alloca ty' => (st, Some (lid, AC_tsubst ty'))
+         | _ => (st, None)
+         end
+       else (st, None)
+    | value_const const5 => (st, None)
+    end
+| _ => (st, None)
+end.
+
+Lemma find_stld_pair_cmd__find_stld_pair_cmd': forall pid st1 c,
+  find_stld_pair_cmd pid st1 c =
+  (let (s, o) := find_stld_pair_cmd' pid st1 c in
+   match o with
+   | ret ac => (s, ac :: snd st1)
+   | merror => (s, snd st1)
+   end).
+Proof.
+  destruct st1 as [s1 acc1].
+  destruct c; simpl; intros; auto.
+    destruct_if; uniq_result; auto.
+
+    destruct value1; auto.
+    destruct_if; auto.
+    destruct s1; auto.
+
+    destruct value2; auto.
+    destruct_if; auto.
+    destruct s1; auto.
+Qed.
+
+Lemma find_stld_pairs_cmds__find_stld_pairs_cmds': forall pid cs st1,
+  fold_left (find_stld_pair_cmd pid) cs st1 =
+  fold_left (fun st c => 
+             match find_stld_pair_cmd' pid st c with
+             | (s, Some ac) => (s, ac::snd st)
+             | (s, None) => (s, snd st)
+             end) cs st1.
+Proof.
+  induction cs as [|c cs]; simpl; intros; auto.
+    rewrite IHcs.
+    f_equal.
+    apply find_stld_pair_cmd__find_stld_pair_cmd'.
+Qed.
+
+(***************************************************************)
+
+Definition wf_cs_actions (acs: AssocList action) (cs:cmds) (pid:id) : Prop :=
+forall acs1 ac acs2 (Heq: acs = acs1 ++ ac :: acs2),
+  wf_cs_action_pre acs1 cs pid ac.
+
+Lemma wf_cs_actions_nil: forall cs pid, wf_cs_actions nil cs pid.
+Proof.
+  unfold wf_cs_actions.
+  intros. symmetry in Heq. contradict Heq. apply app_cons_not_nil.
+Qed.
+
+(***************************************************************)
+
+Definition wf_block_action (acs: AssocList action) (b:block) (pid:id) 
+  : Prop :=
+let '(_, stmts_intro _ cs _) := b in
+wf_cs_actions acs cs pid.
+
+(***************************************************************)
+
+Definition wf_actions (bs:blocks) (pid:id) (rd:list l) (acs: AssocList action) 
+  : Prop :=
+forall acs1 ac acs2 (Heq: acs = acs1 ++ ac :: acs2),
+  exists l0, exists ps0, exists cs0, exists tmn0,
+    In (l0, stmts_intro ps0 cs0 tmn0) bs /\ In l0 rd /\
+    wf_cs_action_pre acs1 cs0 pid ac.
+
+(***************************************************************)
+
+Definition wf_stld_state (cs:cmds) (pid:id) (elt :stld_state * AssocList action)
+  : Prop :=
+let '(s, acs) := elt in
+match s with
+| STLD_init => alloca_in_cmds pid cs = false /\ store_in_cmds pid cs = false
+| STLD_store id0 v0 =>
+    exists cs1 : list cmd, exists ty0 : typ, exists al0 : align, exists cs2, 
+      cs = cs1 ++ insn_store id0 ty0 v0 (value_id pid) al0 :: cs2 /\
+      store_in_cmds pid cs2 = false /\ loads_must_be_in_pre acs pid cs2
+| STLD_alloca t0 =>
+    exists cs1, exists num, exists al, exists cs2, 
+      cs = cs1 ++ insn_alloca pid t0 num al :: cs2 /\
+      store_in_cmds pid cs2 = false /\ loads_must_be_in_pre acs pid cs2
+end.
+
+Lemma wf_stld_state_append: forall st cs1 pid c 
+  (Hwf: wf_stld_state cs1 pid st)
+  (Hnot: alloca_in_cmd pid c = false /\ 
+         store_in_cmd pid c = false /\ 
+         load_in_cmd pid c = false),
+  wf_stld_state (cs1 ++ [c]) pid st.
+Proof.
+  intros.
+  destruct st as [s acs].
+  destruct Hnot as [J1 [J2 J3]].
+  destruct s; simpl in *.
+    destruct Hwf.
+    split.
+      apply alloca_in_cmds_merge; auto.
+      apply store_in_cmds_merge; auto.
+
+    destruct Hwf as [cs2 [t0 [al0 [cs3 [EQ [G1 G2]]]]]]; subst.
+    exists cs2. exists t0. exists al0. exists (cs3 ++ [c]).
+    simpl_env.
+    split; auto.
+    split.
+      apply store_in_cmds_merge; auto.
+      apply loads_must_be_in_pre_append; auto.
+
+    destruct Hwf as [cs2 [num0 [al0 [cs3 [EQ [G1 G2]]]]]]; subst.
+    exists cs2. exists num0. exists al0. exists (cs3 ++ [c]).
+    simpl_env.
+    split; auto.
+    split.
+      apply store_in_cmds_merge; auto.
+      apply loads_must_be_in_pre_append; auto.
+Qed.
+
+Ltac wf_stld_state_append_tac :=
+  try solve 
+    [apply wf_stld_state_append; simpl; try solve [auto | destruct_dec]].
+
+(***************************************************************)
+
+Lemma find_stld_pair_cmd__wf_stld_state: forall (pid : id) cs c st
+  (Hwfst: wf_stld_state cs pid st),
+  wf_stld_state (cs++[c]) pid (find_stld_pair_cmd pid st c).
+Proof.
+  intros.
+  destruct st as [s acs].
+  destruct c; wf_stld_state_append_tac; simpl.
+    Case "1".        
+      destruct (id_dec pid id5); wf_stld_state_append_tac.
+        subst id5. simpl.
+        exists cs. exists value5. exists align5. exists nil.
+        unfold loads_must_be_in_pre, store_in_cmds. auto.
+    Case "2".
+      destruct value1 as [qid|]; wf_stld_state_append_tac.
+      destruct (id_dec pid qid); wf_stld_state_append_tac.
+        subst qid.
+        destruct s.
+        SCase "2.1".
+          simpl in *. destruct Hwfst.
+          split.
+            apply alloca_in_cmds_merge; auto.
+            apply store_in_cmds_merge; auto.
+        SCase "2.2".
+          simpl in *.
+          destruct Hwfst as [cs3 [ty0 [al0 [cs4 [EQ [Hnst Hnld]]]]]]; subst.
+          exists cs3. exists ty0. exists al0.
+          exists (cs4++[insn_load id5 typ5 (value_id pid) align5]).
+          simpl_env. 
+          split; auto.
+          split.
+            apply store_in_cmds_merge; auto.
+            apply loads_must_be_in_pre_append'; auto.
+              simpl. destruct_dec.
+        SCase "2.3".
+          simpl in *.
+          destruct Hwfst as [cs3 [num0 [al0 [cs4 [EQ [Hnst Hnld]]]]]]; subst.
+          exists cs3. exists num0. exists al0. 
+          exists (cs4++[insn_load id5 typ5 (value_id pid) align5]).
+          simpl_env. 
+          split; auto.
+          split.
+            apply store_in_cmds_merge; auto.
+            apply loads_must_be_in_pre_append'; auto.
+              simpl. destruct_dec.
+    Case "3".
+      destruct value2 as [qid|]; wf_stld_state_append_tac.
+      destruct (id_dec pid qid); wf_stld_state_append_tac.
+        subst qid.
+        destruct s.
+        SCase "3.1".
+          simpl. exists cs. exists typ5. exists align5. exists nil.
+          unfold loads_must_be_in_pre, store_in_cmds. auto.
+        SCase "3.2".
+          simpl in *.
+          destruct Hwfst as [cs3 [ty0 [al0 [cs4 [EQ [Hnst Hnld]]]]]]; subst.
+          exists (cs3 ++ insn_store i0 ty0 v (value_id pid) al0 :: cs4). 
+          exists typ5. exists align5. exists nil.
+          simpl_env. 
+          split; auto.
+          split; auto.
+            constructor.
+        SCase "3.3".
+          simpl in *.
+          destruct Hwfst as [cs3 [num0 [al0 [cs4 [EQ [Hnst Hnld]]]]]]; subst.
+          exists (cs3 ++ insn_alloca pid t num0 al0 :: cs4). 
+          exists typ5. exists align5. exists nil.
+          simpl_env. 
+          split; auto.
+          split; auto.
+            constructor.
+Qed.
+
+Lemma find_stld_pairs_cmds__wf_stld_state_aux: forall (pid : id) cs 
+  cs2 cs1 st1 (Heq: cs = cs1 ++ cs2)
+  (Hwfst: wf_stld_state cs1 pid st1),
+  wf_stld_state cs pid (fold_left (find_stld_pair_cmd pid) cs2 st1).
+Proof.
+  induction cs2 as [|c2 cs2]; simpl; intros; subst; auto.
+    simpl_env. auto.
+
+    apply IHcs2 with (cs3:=cs1++[c2]); simpl_env; auto.
+    clear IHcs2.
+    apply find_stld_pair_cmd__wf_stld_state; auto.
+Qed.
+
+Lemma find_stld_pairs_cmds__wf_stld_state: forall (pid : id) cs,
+  wf_stld_state cs pid (fold_left (find_stld_pair_cmd pid) cs (STLD_init, nil)).
+Proof.
+  intros.
+  assert (cs = nil ++ cs) as EQ. auto.
+  eapply find_stld_pairs_cmds__wf_stld_state_aux in EQ; eauto.
+  simpl. unfold alloca_in_cmds, store_in_cmds. auto.
+Qed.
+
+Lemma find_stld_pair_cmd'__wf_cs_action_pre: forall cs cs1 c cs2 st1 st2 pid 
+  (Heq: cs = cs1 ++ c :: cs2)
+  (Huniq: NoDup (getCmdsLocs cs))
+  (Hwfst1: wf_stld_state cs1 pid st1) ac
+  (Hfind: find_stld_pair_cmd' pid st1 c = (st2, Some ac)),
+  wf_cs_action_pre (snd st1) cs pid ac.
+Proof.
+
+Ltac find_stld_pair_cmd'__wf_cs_action_pre_tac :=
+  match goal with
+  | Huniq: NoDup _ |- context [(?A ++ ?b :: ?C) ++ ?d :: ?E] =>
+    rewrite_env (A++b::(C++d::E));
+    rewrite_env (A++b::(C++d::E)) in Huniq;
+    exists C; exists d; exists E; exists (getCmdsLocs A)
+  end.
+
+  intros. subst.
+  destruct st1 as [s1 acc1]. 
+  destruct c; simpl in Hfind; tinv Hfind.
+  Case "1".
+    destruct_if; tinv Hfind.
+  Case "2".
+    destruct value1; tinv Hfind.
+    destruct_if.
+    destruct s1; inv H0.
+    SCase "2.1".
+      simpl in *.
+      destruct Hwfst1 as [cs3 [ty0 [al0 [cs4 [EQ [Hnst Hnld]]]]]]; subst.
+      exists i0. 
+      find_stld_pair_cmd'__wf_cs_action_pre_tac.
+      split.
+        rewrite getCmdsLocs_app in Huniq. simpl in Huniq.
+        apply find_init_stld_inl_intro; auto.
+      split; auto.
+      split; auto.
+      split; simpl; auto.
+        destruct_dec.
+    SCase "2.2".
+      simpl in *.
+      destruct Hwfst1 as [cs3 [num0 [al0 [cs4 [EQ [Hnst Hnld]]]]]]; subst.
+      find_stld_pair_cmd'__wf_cs_action_pre_tac.
+      split.
+        rewrite getCmdsLocs_app in Huniq. simpl in Huniq.
+        apply find_init_stld_inr_intro; auto.
+      split; auto.
+      split; auto.
+      split; simpl; auto.
+        destruct_dec.
+  Case "3".
+    destruct value2; tinv Hfind.
+    destruct_if.
+    destruct s1; inv H0.
+    simpl in *.
+    destruct Hwfst1 as [cs3 [ty0 [al0 [cs4 [EQ [Hnst Hnld]]]]]]; subst.
+    exists v. 
+    find_stld_pair_cmd'__wf_cs_action_pre_tac.
+    split.
+      rewrite getCmdsLocs_app in Huniq. simpl in Huniq.
+      apply find_init_stld_inl_intro; auto.
+    split; auto.
+    split; simpl; auto.
+      destruct_dec.
+Qed.
+
+Local Opaque find_stld_pair_cmd' find_stld_pair_cmd.
+
+Lemma find_stld_pairs_cmds_cons_inv: forall pid cs s acs s' acs'
+  (Heq: fold_left (find_stld_pair_cmd pid) cs (s, acs) = (s', acs')),
+  exists acs0, acs' = acs0 ++ acs.
+Proof.
+  induction cs as [|c cs]; simpl; intros.
+    uniq_result. exists nil. auto.
+
+    rewrite find_stld_pair_cmd__find_stld_pair_cmd' in Heq.
+    case_eq (find_stld_pair_cmd' pid (s, acs) c).
+    intros s0 o Heq'.
+    rewrite Heq' in Heq.
+    destruct o as [ac'|]; simpl in Heq. 
+      apply IHcs in Heq.
+      destruct Heq as [acs0 Heq]; subst.
+      exists (acs0 ++ [ac']). simpl_env. auto.
+    
+      apply IHcs in Heq; auto.
+Qed.
+
+Lemma find_stld_pairs_cmds__split_aux: forall pid cs acs1 ac acs2 s0 acs0 s2
+  (Heq: fold_left (find_stld_pair_cmd pid) cs (s0, acs0) = 
+          (s2, acs2 ++ ac :: acs1 ++ acs0)),
+  exists cs1, exists c, exists cs2, exists s1, exists s,
+    cs = cs1 ++ c :: cs2 /\
+    fold_left (find_stld_pair_cmd pid) cs1 (s0, acs0) = (s1, acs1 ++ acs0) /\
+    find_stld_pair_cmd' pid (s1, acs1 ++ acs0) c = (s, Some ac) /\    
+    fold_left (find_stld_pair_cmd pid) cs2 (s, ac::acs1 ++ acs0) = 
+      (s2, acs2 ++ ac :: acs1 ++ acs0).
+Proof.
+  induction cs as [|c cs]; simpl; intros; subst.
+  Case "base".
+    inversion Heq. anti_simpl_env.  
+  Case "ind".
+    rewrite find_stld_pair_cmd__find_stld_pair_cmd' in Heq.
+    case_eq (find_stld_pair_cmd' pid (s0, acs0) c).
+    intros s o Heq'.
+    rewrite Heq' in Heq.
+    destruct o as [ac'|]; simpl in Heq. 
+    SCase "1".
+      assert (J:=Heq).
+      apply find_stld_pairs_cmds_cons_inv in J. destruct J as [acs3 J].
+      anti_simpl_env.
+      destruct acs1 as [|ac1 acs1].
+      SSCase "1.1".
+        anti_simpl_env.
+        exists nil. exists c. exists cs. exists s0. exists s. 
+        split; auto.
+      SSCase "1.2".
+        destruct (cons_last _ ac1 acs1) as [pre [last EQ]].
+        rewrite EQ in J, Heq.
+        anti_simpl_env. 
+        rewrite_env (acs2 ++ ac :: pre ++ (ac' :: acs0)) in Heq.
+        apply IHcs in Heq; auto.
+        destruct Heq as [cs1 [c' [cs2 [s1 [s3 [J1 [J2 [J3 J4]]]]]]]].
+        exists (c::cs1). exists c'. exists cs2. exists s1. exists s3. 
+        split.
+          simpl. subst. auto.
+        split.
+          simpl. rewrite find_stld_pair_cmd__find_stld_pair_cmd'. rewrite Heq'.      
+          rewrite_env (([ac1] ++ acs1) ++ acs0). rewrite EQ. simpl_env. auto.
+        split.
+          rewrite_env (([ac1] ++ acs1) ++ acs0). rewrite EQ. simpl_env. auto.
+          rewrite_env (([ac1] ++ acs1) ++ acs0). rewrite EQ. simpl_env. auto.
+
+    SCase "2".
+      apply IHcs in Heq; auto.
+      destruct Heq as [cs1 [c' [cs2 [s1 [s3 [J1 [J2 [J3 J4]]]]]]]].
+      exists (c::cs1). exists c'. exists cs2. exists s1. exists s3.
+      simpl. rewrite find_stld_pair_cmd__find_stld_pair_cmd'. rewrite Heq'.      
+      subst; split; auto.
+Qed.
+
+Lemma find_stld_pairs_cmds__split: forall pid cs acs1 ac acs2 s2
+  (Heq: fold_left (find_stld_pair_cmd pid) cs (STLD_init, nil) = 
+          (s2, acs2 ++ ac :: acs1)),
+  exists cs1, exists c, exists cs2, exists s1, exists s, 
+    cs = cs1 ++ c :: cs2 /\
+    fold_left (find_stld_pair_cmd pid) cs1 (STLD_init, nil) = (s1, acs1) /\
+    find_stld_pair_cmd' pid (s1, acs1) c = (s, Some ac) /\    
+    fold_left (find_stld_pair_cmd pid) cs2 (s, ac::acs1) = 
+      (s2, acs2 ++ ac :: acs1).
+Proof.
+  intros.
+  replace acs1 with (acs1++nil) in Heq; auto.
+  apply find_stld_pairs_cmds__split_aux in Heq.
+  simpl_env in *. auto.
+Qed.
+
+Transparent find_stld_pair_cmd' find_stld_pair_cmd.
+
+Lemma find_stld_pairs_cmds__wf_cs_actions: forall pid cs 
+  (Huniq: NoDup (getCmdsLocs cs)),
+  wf_cs_actions (find_stld_pairs_cmds cs pid) cs pid.
+Proof.
+  unfold find_stld_pairs_cmds.
+  intros.
+  intros acs1 ac acs2 Heq.
+  case_eq (fold_left (find_stld_pair_cmd pid) cs (STLD_init, nil)).
+  intros s' ac' Hfind.
+  rewrite Hfind in Heq. simpl in Heq.
+  assert (ac' = rev acs2 ++ ac :: rev acs1) as EQ.
+    rewrite <- rev_involutive with (l:=ac').
+    rewrite Heq. rewrite rev_app_distr. simpl. simpl_env. auto.
+  subst. clear Heq.
+  apply find_stld_pairs_cmds__split in Hfind.
+  destruct Hfind as [cs1 [c [cs2 [s1 [s [J1 [J2 [J3 J4]]]]]]]].
+  eapply find_stld_pair_cmd'__wf_cs_action_pre in J3; eauto.
+    simpl in J3. apply wf_cs_action_pre_rev; auto.
+
+    rewrite <- J2. apply find_stld_pairs_cmds__wf_stld_state; auto.
+Qed.
+
+Lemma find_stld_pairs_block__wf_cs_actions: forall pid rd b
+  (Huniq: NoDup (getStmtsLocs (snd b))),
+  wf_block_action (find_stld_pairs_block pid rd b) b pid.
+Proof.
+  destruct b as [? [? cs ?]]. simpl. intros.
+  destruct_if; auto using wf_cs_actions_nil.
+  split_NoDup.
+  apply find_stld_pairs_cmds__wf_cs_actions; auto.
+Qed.
+
+Lemma find_stld_pairs_blocks__split: forall pid rd bs acs1 ac acs2
+  (Hmap: flat_map (find_stld_pairs_block pid rd) bs = acs1 ++ ac :: acs2),
+  exists b, exists bs1, exists bs2,
+  exists acs11, exists acs12, exists acs21, exists acs22,
+    bs = bs1 ++ b :: bs2 /\
+    acs1 = acs11 ++ acs12 /\
+    acs2 = acs21 ++ acs22 /\
+    find_stld_pairs_block pid rd b = acs12 ++ ac :: acs21 /\
+    flat_map (find_stld_pairs_block pid rd) bs1 = acs11 /\
+    flat_map (find_stld_pairs_block pid rd) bs2 = acs22.
+Proof.
+  induction bs as [|b bs]; simpl; intros.
+    symmetry in Hmap. contradict Hmap. apply app_cons_not_nil.
+
+    apply app_split in Hmap.
+    destruct Hmap as [[u1 [u2 [J1 [J2 J3]]]]|[z1 [z2 [J1 [J2 J3]]]]].
+      exists b. exists nil. exists bs. exists nil. exists acs1. 
+      exists u1. exists u2. simpl. eauto 10.
+
+      apply_clear IHbs in J2.
+      destruct J2 as 
+        [b0 [bs1 [bs2 [acs11 [acs12 [acs21 [acs22 [J2 
+          [J7 [J4 [J5 [J6 J8]]]]]]]]]]]]; subst.
+      exists b0. exists (b::bs1). exists bs2.
+      exists (find_stld_pairs_block pid rd b ++ 
+              flat_map (find_stld_pairs_block pid rd) bs1).
+      exists acs12. exists acs21.
+      exists (flat_map (find_stld_pairs_block pid rd) bs2).
+      simpl_env. split; auto.
+Qed.
+
+Lemma find_stld_pairs_block__reach: forall pid rd l0 sts0
+  acs1 ac acs2
+  (Hfind: find_stld_pairs_block pid rd (l0, sts0) =
+            acs1 ++ ac :: acs2),
+  In l0 rd.
+Proof.
+  simpl. intros.
+  destruct_if; auto.
+    symmetry in H0. contradict H0. destruct sts0. apply app_cons_not_nil.
+Qed.
+
+Lemma find_stld_pairs_blocks__wf_actions: forall pid rd bs actions
+  (Huniq: NoDup (getBlocksLocs bs))
+  (Hfind: actions = flat_map (find_stld_pairs_block pid rd) bs),
+  wf_actions bs pid rd actions.
+Proof.
+  intros.
+  unfold wf_actions.
+  intros. subst.
+  apply find_stld_pairs_blocks__split in Heq.
+  destruct Heq as 
+    [b [bs1 [bs2 [acs11 [acs12 [acs21 [acs22 
+      [J1 [J2 [J3 [J4 [J5 J6]]]]]]]]]]]]; subst.
+  destruct b as [l0 [ps0 cs0 tmn0]].
+  exists l0. exists ps0. exists cs0. exists tmn0.
+  split. xsolve_in_list.
+  split. apply find_stld_pairs_block__reach in J4; auto.
+    simpl in J4.
+    destruct_if.
+      apply wf_cs_action_pre_weaken.
+      rewrite getBlocksLocs_app in Huniq. simpl in Huniq.
+      split_NoDup. 
+      apply find_stld_pairs_cmds__wf_cs_actions with (pid:=pid) in Huniq; auto.
+      apply Huniq in H0; auto.
+
+      symmetry in H0. contradict H0. apply app_cons_not_nil.
+Qed.
+
+(***************************************************************)
+
 Definition subst_action_action (ac:action) (elt:id * action): action :=
 let '(id1, ac1) := elt in
 match action2value ac1 with
 | Some v1 => subst_action id1 v1 ac
 | _ => ac
 end.
+
+Lemma list_subst_actions_cons_inv: forall id0 ac0 acs id1 ac1' acs2'
+  (Heq: ListComposedPass.subst_actions id0 ac0 acs = (id1, ac1') :: acs2'),
+  exists ac1, exists acs2,
+    acs = (id1, ac1) :: acs2 /\ 
+    subst_action_action ac1 (id0, ac0)= ac1' /\
+    ListComposedPass.subst_actions id0 ac0 acs2 = acs2'.
+Proof.
+  unfold ListComposedPass.subst_actions.
+  intros.
+  case_eq (action2value ac0).
+    intros v Heqv. rewrite Heqv in Heq.
+    unfold ListMap.map in *.
+    apply map_cons_inv in Heq; auto.
+    destruct Heq as [[] [x2 [EQ [J1 J2]]]]; subst.
+    inv J2.
+    exists a0. exists x2.
+    split; auto.
+    split; auto.
+      unfold subst_action_action, subst_action.
+      rewrite Heqv. auto.
+
+    intros Heqv. rewrite Heqv in Heq.
+    subst. 
+    unfold subst_action_action. rewrite Heqv. eauto.
+Qed.
+
+(***************************************************************)
 
 Definition pipelined_actions_action (actions: list (id*action)) (ac:action) 
   : action :=
@@ -308,7 +1655,6 @@ Definition composed_pipelined_actions (pairs: AssocList action) (f:fdef): fdef :
 ListComposedPass.substs_fdef 
   (pipelined_actions__composed_actions (substs_actions pairs)) f.
 
-
 (***************************************************************)
 
 Require Import Paths.
@@ -328,15 +1674,371 @@ fun (arc:Arc) =>
   In (n2, AC_vsubst (value_id n1)) actions. 
 
 Definition acyclic_actions : Prop :=
-  forall x y vl al p,
-    Cycle avertexes aarcs x y vl al p -> vl = V_nil.
+  forall x y vl al p (Hcyc: Cycle avertexes aarcs x y vl al p), 
+    vl = V_nil.
 
 End ActionGraph.
 
-Lemma find_stld_pairs_blocks_acyclic: forall pid rd bs actions
+(* go to typings_props.v *)
+Lemma idDominates_trans: forall s m f (HwfF:wf_fdef s m f)
+  (HuniqF: uniqFdef f) id1 id2 id3
+  (Hdom1: idDominates f id1 id2) (Hdom2: idDominates f id2 id3),
+  idDominates f id1 id3.
+Proof.
+  unfold idDominates, inscope_of_id.
+  intros.
+  inv_mbind.
+  symmetry_ctx.
+  assert (blockInFdefB (l3,s1) f = true) as HBinF0.
+    solve_blockInFdefB.
+  assert (blockInFdefB (l1,s0) f = true) as HBinF1.
+    solve_blockInFdefB.
+  destruct s1 as [ps2 cs2 tmn2].
+  destruct s0 as [ps3 cs3 tmn3].
+  apply fold_left__spec in HeqR2.
+  apply fold_left__spec in HeqR0.
+  destruct HeqR2 as [_ [_ HeqR2]].
+  destruct HeqR0 as [Hinit0 [_ HeqR0]].
+  apply_clear HeqR2 in Hdom1.
+  apply_clear HeqR0 in Hdom2.
+  assert (~ In id3 (getArgsIDsOfFdef f)) as Hnotin1.
+    solve_notin_getArgsIDs.
+  assert (~ In id2 (getArgsIDsOfFdef f)) as Hnotin2.
+    solve_notin_getArgsIDs.
+  assert (In id2 (getStmtsLocs (stmts_intro ps2 cs2 tmn2))) as Hin9.
+    solve_in_list.
+  assert (In id3 (getStmtsLocs (stmts_intro ps3 cs3 tmn3))) as Hin10.
+    solve_in_list.
+  destruct Hdom1 as [Hdom1 | [sts1 [a1 [J1 [J2 J3]]]]].
+  Case "local".
+    unfold init_scope in Hdom1.
+    destruct_if.
+    SCase "in args". 
+      admit.
+    SCase "not in args".
+      destruct Hdom2 as [Hdom2 | [sts2 [a2 [J4 [J5 J6]]]]].
+      SSCase "local".
+        unfold init_scope in Hdom2.
+        destruct_if; try tauto.
+(*
+        assert (NoDup (getCmdsLocs cs3)) as Hnodup.
+          solve_NoDup.
+        assert (In id2 (cmds_dominates_cmd cs3 id3)) as Hin2.
+          apply in_app_or in Hdom2.
+          destruct Hdom2 as [Hdom2 | Hdom2]; try solve [contradict Hdom2; auto].
+          apply in_app_or in Hdom2.
+          destruct Hdom2 as [Hdom2 | Hdom2]; try solve [contradict Hdom2; auto].
+          auto.
+        assert (In id1 (cmds_dominates_cmd cs3 id2)) as Hin1.
+          apply in_app_or in Hdom1.
+          destruct Hdom1 as [Hdom1 | Hdom1]; try solve [contradict Hdom1; auto].
+          apply in_app_or in Hdom1.
+          destruct Hdom1 as [Hdom1 | Hdom1]; try solve [contradict Hdom1; auto].
+          auto.
+        assert (In id1 (getCmdsLocs cs3) /\ In id2 (getCmdsLocs cs3)) as Hin.
+          apply cmds_dominates_cmd_spec in Hin2.
+          apply cmds_dominates_cmd_spec in Hin1.
+          split; solve_in_list.
+        destruct Hin as [Hin3 Hin4].
+        eapply cmds_dominates_cmd_acyclic; eauto.
+*)
+        admit.
+      SSCase "remote".
+        admit.
+(*
+        apply ListSet.set_diff_elim2 in J4; auto.
+        simpl in J4. auto.
+*)
+  Case "remote".
+    admit.
+(*
+      assert ((a1, sts1) = (l1, stmts_intro ps3 cs3 tmn3)) as EQ.
+        eapply block_eq2 with (id1:=id1); eauto 1.
+          solve_blockInFdefB.
+          solve_in_list.
+      inv EQ.
+      apply lookupBlockViaLabelFromFdef_inv in J2; auto.
+      destruct J2; subst.
+      destruct Hdom2 as [Hdom2 | [sts2 [a2 [J4 [J5 J6]]]]].
+      SCase "local".
+        unfold init_scope in Hdom2.
+        destruct_if; try tauto.
+        assert ((l3, stmts_intro ps2 cs2 tmn2) =
+                (l1, stmts_intro ps3 cs3 tmn3)) as EQ.
+          eapply block_eq2 with (id1:=id2); eauto 1.
+            simpl.
+            solve_in_list.
+            apply cmds_dominates_cmd_spec in Hdom2.
+            solve_in_list.
+        inv EQ.
+        apply ListSet.set_diff_elim2 in J1; auto.
+        simpl in J1. auto.
+      SCase "remote".
+        assert ((a2, sts2) = (l3, stmts_intro ps2 cs2 tmn2)) as EQ.
+          eapply block_eq2 with (id1:=id2); eauto 1.
+            solve_blockInFdefB.
+            solve_in_list.
+        inv EQ.
+        apply lookupBlockViaLabelFromFdef_inv in J5; auto.
+        assert (l3 <> l1) as Hneq.
+          intro J. subst.
+          apply ListSet.set_diff_elim2 in J4; auto.
+          simpl in J4. auto.
+        eapply sdom_acyclic in Hneq; eauto 1.
+          apply ListSet.set_diff_elim1 in J4; auto.
+          apply ListSet.set_diff_elim1 in J1; auto.
+*)
+Qed.
+
+Require Import Program.Tactics.
+
+Lemma wf_actions__in: forall bs pid rd acs ac
+  (Hwfa: wf_actions bs pid rd acs) (Hin: In ac acs),
+  exists acs1, exists acs2,
+  exists l0, exists ps0, exists cs0, exists tmn0,
+    acs = acs1 ++ ac :: acs2 /\
+    In (l0, stmts_intro ps0 cs0 tmn0) bs /\ In l0 rd /\
+    wf_cs_action_pre acs1 cs0 pid ac.
+Proof.
+  intros.
+  apply in_split in Hin.
+  destruct Hin as [acs1 [acs2 Hin]].
+  assert (J:=Hin).
+  apply Hwfa in J. destruct_conjs. eauto 10.
+Qed.
+
+Lemma find_stld_pairs_block__reach': forall (fh : fheader) (bs : blocks)
+  (HuniqF : uniqFdef (fdef_intro fh bs)) (pid : id) (rd : list l) (id0 : atom)
+  (Hin : id0 `in` dom (flat_map (find_stld_pairs_block pid rd) bs)),
+  exists l0 : l, exists sts0 : stmts,
+    blockInFdefB (l0, sts0) (fdef_intro fh bs) /\
+    In id0 (getStmtsLocs sts0) /\
+    In l0 rd.
+Proof.
+  intros.
+  apply binds_In_inv in Hin.
+  destruct Hin as [a Hin].
+  unfold binds in Hin.
+  apply in_flat_map in Hin.
+  destruct Hin as [b [Hin1 Hin2]].
+  assert (J:=Hin2).
+  apply binds_In in J.
+  apply find_stld_pairs_block__incl in J.
+  destruct b as [l0 sts0].
+  exists l0. exists sts0.
+  split. simpl. solve_in_list.
+  split; auto.
+    apply in_split in Hin2.
+    destruct Hin2 as [l1 [l2 Hfind]].   
+    apply find_stld_pairs_block__reach in Hfind; auto.
+Qed.
+
+Lemma find_stld_pairs_block__reach'': forall (fh : fheader) (bs : blocks)
+  (HuniqF : uniqFdef (fdef_intro fh bs)) (pid : id) (rd : list l) (id0 : atom)
+  (l0 : l) (sts0 : stmts)
+  (H : lookupBlockViaIDFromFdef (fdef_intro fh bs) id0 = ret (l0, sts0))
+  (Hin : id0 `in` dom (flat_map (find_stld_pairs_block pid rd) bs)),
+  In l0 rd.
+Proof.
+  intros.
+  eapply find_stld_pairs_block__reach' in Hin; eauto.
+  destruct Hin as [l1 [sts1 [J1 [J2 J3]]]].
+  assert (J':=H).
+  apply lookupBlockViaIDFromBlocks__InGetBlockIDs in J'.
+  apply in_getStmtsIDs__in_getStmtsLocs in J'.
+  assert ((l1, sts1) = (l0, sts0)) as EQ.
+    eapply block_eq2; eauto 1.
+      solve_blockInFdefB.
+  inv EQ. auto.
+Qed.
+
+Lemma find_stld_pairs_block__isReachableFromEntry: forall s m fh bs 
+  (HwfF:wf_fdef s m (fdef_intro fh bs))
+  (HuniqF: uniqFdef (fdef_intro fh bs)) pid rd actions
+  (Hreach: ret rd = reachablity_analysis (fdef_intro fh bs))
   (Hfind: actions = flat_map (find_stld_pairs_block pid rd) bs),
+  forall id0 (a:avertexes actions (index id0)) (b : block),
+  lookupBlockViaIDFromFdef (fdef_intro fh bs) id0 = ret b ->
+  isReachableFromEntry (fdef_intro fh bs) b.
+Proof.
+  intros. destruct b as [l0 sts0].
+  eapply reachablity_analysis__reachable; eauto.
+  subst. 
+  destruct a as [Hin | Hin].
+  Case "1".
+    eapply find_stld_pairs_block__reach''; eauto.
+  Case "2".
+    destruct Hin as [id1 Hin].
+    assert (Hin':=Hin).
+    apply binds_In in Hin'.
+    eapply find_stld_pairs_block__reach' in Hin'; eauto.
+    destruct Hin' as [l1 [sts1 [J1 [J2 J3]]]].
+    assert (Huniq:=HuniqF).
+    apply uniqF__uniqBlocksLocs in Huniq.    
+    remember (flat_map (find_stld_pairs_block pid rd) bs) as acs.
+    apply find_stld_pairs_blocks__wf_actions in Heqacs; auto.
+    eapply wf_actions__in in Hin; eauto.
+    destruct Hin as 
+      [acs1 [acs2 [l2 [ps0 [cs0 [tmn0 [EQ [Hin1 [Hin2 Hwf]]]]]]]]]; subst.
+    simpl in Hwf.
+    destruct Hwf as [id2 [cs01 [c0 [cs02 [dones [J6 [J7 [J8 [J4 J5]]]]]]]]].
+    apply find_init_stld_inl_spec in J6.
+    destruct J6 as [cs1 [ty [al J6]]]; subst.
+    remember (insn_store id2 ty (value_id id0) (value_id pid) al) as c1.
+    remember (l2, stmts_intro ps0
+               (cs1 ++ c1 :: cs01 ++ c0 :: cs02) tmn0) as b.
+    remember (fdef_intro fh bs) as f.
+    assert (exists ids1, Some ids1 = inscope_of_cmd f b c1) as R1.
+      assert (J:=inscope_of_cmd__total f b c1).
+      destruct (inscope_of_cmd f b c1); eauto.
+      congruence.
+    destruct R1 as [ids1 R1].
+    assert (blockInFdefB b f = true) as HBInF.
+      subst f. simpl. solve_in_list.
+    assert (cmdInBlockB c1 b = true) as HC1InB.
+      subst. solve_in_list.
+    assert (isReachableFromEntry f b) as Hreach'.
+      subst b. simpl.
+      eapply reachablity_analysis__reachable; eauto.
+    assert (In id0 (getCmdOperands c1)) as Hinops.
+      subst c1. simpl. auto.
+    assert (J:=R1).
+    eapply cmd_operands__in_scope' with (id1:=id0) in J; eauto 1.
+    subst b. 
+    eapply inscope_of_cmd__id_in_reachable_block in R1; eauto.
+      apply R1 in H. simpl in H.
+      eapply reachable__reachablity_analysis; eauto.
+      
+      solve_in_list.
+Qed.
+
+Lemma find_stld_pairs_blocks__idDominates: forall s m fh bs 
+  (HwfF:wf_fdef s m (fdef_intro fh bs))
+  (HuniqF: uniqFdef (fdef_intro fh bs)) actions rd pid
+  (Hreach: ret rd = reachablity_analysis (fdef_intro fh bs))
+  (Hfind: actions = flat_map (find_stld_pairs_block pid rd) bs) id1 id2
+  (Hin: In (id1, AC_vsubst (value_id id2)) actions),
+  idDominates (fdef_intro fh bs) id2 id1.
+Proof.
+  intros.
+  assert (Huniq:=HuniqF).
+  apply uniqF__uniqBlocksLocs in Huniq.
+  assert (J:=Hfind).
+  apply find_stld_pairs_blocks__wf_actions in J; auto.
+  eapply wf_actions__in in J; eauto.
+  destruct J as 
+    [acs1 [acs2 [l0 [ps0 [cs0 [tmn0 [EQ [Hin1 [Hin2 Hwf]]]]]]]]]; subst.
+  simpl in Hwf.
+  destruct Hwf as [id0 [cs01 [c0 [cs02 [dones [J1 [J2 [J3 [J4 J5]]]]]]]]].
+  apply find_init_stld_inl_spec in J1.
+  destruct J1 as [cs1 [ty [al J1]]]; subst.
+  remember (l0, stmts_intro ps0
+             (cs1 ++
+              insn_store id0 ty (value_id id2) (value_id pid) al
+              :: cs01 ++ c0 :: cs02) tmn0) as b.
+  remember (insn_store id0 ty (value_id id2) (value_id pid) al) as c1.
+  remember (fdef_intro fh bs) as f.
+  assert (getCmdID c0 <> merror) as Hmerror.
+    destruct c0; inv J4. simpl. congruence.
+  assert (isReachableFromEntry f b) as Hreach'.
+    subst f.
+    eapply find_stld_pairs_block__isReachableFromEntry 
+      with (pid:=pid)(id0:=getCmdLoc c0); eauto 1.
+      simpl. left. simpl_env. eapply binds_In; eauto.
+
+      assert (insnInFdefBlockB (insn_cmd c0) (fdef_intro fh bs) b = true) 
+        as Hin'.
+        subst. simpl. apply andb_true_iff.
+        split; solve_in_list.
+      solve_lookupBlockViaIDFromFdef.
+  assert (blockInFdefB b f = true) as HBInF.
+    subst f. simpl. solve_in_list.
+  assert (cmdInBlockB c0 b = true) as HC0InB.
+    subst. solve_in_list.
+  assert (cmdInBlockB c1 b = true) as HC1InB.
+    subst. solve_in_list.
+  assert (exists ids1, Some ids1 = inscope_of_cmd f b c1) as R1.
+    assert (J:=inscope_of_cmd__total f b c1).
+    destruct (inscope_of_cmd f b c1); eauto.
+    congruence.
+  destruct R1 as [ids1 R1].
+  assert (exists ids0, Some ids0 = inscope_of_cmd f b c0) as R0.
+    assert (J:=inscope_of_cmd__total f b c0).
+    destruct (inscope_of_cmd f b c0); eauto.
+    congruence.
+  destruct R0 as [ids0 R0].
+  eapply inscope_of_cmd__idDominates; eauto 1.
+    assert (AtomSet.set_eq (ids1 ++ getCmdsIDs (c1::cs01)) ids0) as EQ'.
+      subst. unfold inscope_of_cmd in *.
+      eapply inscope_of_id__append_cmds; eauto.
+        solve_NoDup.
+    eapply cmd_operands__in_scope' with (id1:=id2) in R1; eauto 1.
+      apply EQ'. solve_in_list.
+      subst c1. simpl. auto.
+Qed.
+
+Lemma find_stld_pairs_blocks__walk_idDominates: forall s m fh bs 
+  (HwfF:wf_fdef s m (fdef_intro fh bs))
+  (HuniqF: uniqFdef (fdef_intro fh bs)) actions rd pid
+  (Hreach: ret rd = reachablity_analysis (fdef_intro fh bs))
+  (Hfind: actions = flat_map (find_stld_pairs_block pid rd) bs)
+  id1 id2 vl al (Hnnil: vl <> V_nil)
+  (Hw: Walk (avertexes actions) (aarcs actions) (index id1) (index id2) vl al),
+  idDominates (fdef_intro fh bs) id2 id1.
+Proof.
+  intros.
+  remember (avertexes actions) as V.
+  remember (aarcs actions) as A.
+  remember (index id1) as x.
+  remember (index id2) as y.
+  generalize dependent id1.
+  generalize dependent id2.
+  induction Hw; intros; subst.
+  Case "1".
+    congruence.
+  Case "2".
+    destruct y as [id3].
+    eapply find_stld_pairs_blocks__idDominates in a; eauto.
+    destruct vl as [|v' vl].
+    SCase "2.1".
+      inv Hw; auto.
+    SCase "2.2".
+      eapply idDominates_trans; eauto 1.
+      apply IHHw; auto. 
+        intro H. inv H.
+Qed.
+
+Lemma find_stld_pairs_blocks_acyclic: forall s m fh bs 
+  (HwfF: wf_fdef s m (fdef_intro fh bs))
+  (HuniqF: uniqFdef (fdef_intro fh bs)) pid rd actions
+  (Hfind: actions = flat_map (find_stld_pairs_block pid rd) bs)
+  (Hreach: ret rd = reachablity_analysis (fdef_intro fh bs)),
   acyclic_actions actions.
-Admitted.
+Proof.
+  unfold acyclic_actions, Cycle.
+  intros. subst.
+  assert (Hwfa:=HuniqF). 
+  apply uniqF__uniqBlocksLocs in Hwfa.
+  apply find_stld_pairs_blocks__wf_actions 
+    with (pid:=pid)(rd:=rd)(actions:=flat_map (find_stld_pairs_block pid rd) bs)
+    in Hwfa; auto.
+  destruct vl as [|v vl]; auto.
+  assert (Hin:=p). apply P_endx_inv in Hin.
+  apply Path_isa_walk in p. 
+  destruct y as [id0].
+  eapply find_stld_pairs_blocks__walk_idDominates in p; eauto.
+  Case "1".
+    eapply idDominates_acyclic in p; eauto.
+    SCase "1.1".
+      inv p.
+    SCase "1.2".
+      intros.
+      eapply find_stld_pairs_block__isReachableFromEntry in Hin; eauto.     
+  Case "2".
+    intro H. inv H.
+Qed.
+
+(***************************************************************)
 
 Lemma list_compose_actions__list_composed_substs: forall actions 
   (Hacyclic: acyclic_actions actions) (Huniq: uniq actions) f,
